$$\begin{gather} 
\delta Q=d U+\delta A \\
d U=\nu RdT \\
\delta A=PdV \\
\delta Q=\nu RdT+PdV =\nu RdT+\frac{\nu RT}{V}dV\\
d w=P(x,y)dx+Q(x,y)dy=\frac{ \partial w }{ \partial x } dx+\frac{ \partial w }{ \partial y } dy \Rightarrow \\
\frac{ \partial P }{ \partial y } =\frac{ \partial ^2w }{ \partial x \partial y }=\frac{ \partial P }{ \partial x } \Rightarrow  \\
\frac{ \partial  }{ \partial V } \nu R=0 \\
\frac{ \partial  }{ \partial T } \frac{\nu RT}{V}=\frac{\nu R}{V}\neq 0\Rightarrow \delta Q\neq dw \\
dS=\frac{\nu R}{T}dT+\frac{P}{T}dV=\frac{\nu R}{T}dT+\frac{\nu R}{V}dV \\
\frac{ \partial  }{ \partial V } \frac{\nu R}{T}=0\\
\frac{ \partial  }{ \partial T } \frac{\nu R}{V}=0
\end{gather}$$

$$\begin{gather}
m\dot{\vec{V}}d\vec{r}=\vec{F}d\vec{r} \\
m\dot{\vec{V}}\vec{V}dt=\vec{F}\vec{V}dt \\
\frac{d(\vec{V}\vec{V})}{dt}=2\dot{\vec{V}}\vec{V} \\
\frac{m}{2}d(\vec{V}\vec{V})=\vec{F}d\vec{r} \\
dA=d\left( \frac{mV^2}{2} \right) \\
A=\frac{mV^2}{2}\vert_{V_{\text{н}}}^{V_{\text{к}}} \\
A=\Delta E_{\text{к}} \\
\delta A=\vec{F}d\vec{r} \\
dE_{\text{п}}=-\delta A \\
\vec{F}=-\operatorname{grad} E_{\text{п}} \\
A=-\Delta E_{\text{п}} \\
A=-\Delta U=\Delta K \\
E=C
\end{gather}$$
$$\begin{gather}
n(U)=n_{0}\cdot \exp\left( -\frac{U}{kT} \right) \\
U=E_{\text{п}}-E_{0} \\
n(E_{0})=n_{0} \\
\frac{n(E_{2})}{n(E_{1})}=\frac{\exp\left( -\frac{E_{2}}{kT} \right)}{\exp\left( -\frac{E_{1}}{kT} \right)}=\exp\left( -\frac{E_{2}-E_{1}}{kT} \right)
\end{gather}$$