

#### 05/04/2025
Условие:
2 Вариант
$$\begin{gather}
\begin{cases}
u_{t}=u_{xx}+u+\left( 3\sin\frac{5\pi x}{4}+ 1\right)e^{t} \ \   (1) \\
u|_{x=0}= te^{t}\\
u_{x}\vert_{x=2}= e^{t}\\
u\vert_{t=0}=x+2
\end{cases} \\
u(x,t)=v(x,t)e^{\beta t}  \\
u_{x}=v_{x}e^{\beta t} \\
u_{t}=e^{\beta t}(v_{t}+\beta v) \\
u_{xx}=v_{xx}e^{\beta t} \\
 \\
(1) \ \ e^{\beta t}(v_{t}+\beta v)=e^{\beta t}(v_{xx}+v)+\left( 3\sin\frac{5\pi x}{4}+ 1\right)e^{t} \ \ (2) \\
\beta=1\Rightarrow u=ve^t\Rightarrow v=ue^{-t} \\
(2)\ \ v_{t}= v_{xx}+3\sin\frac{5\pi x}{4}+ 1 \ \ (3)\\
\begin{cases}
v_{t}= v_{xx}+3\sin\frac{5\pi x}{4}+ 1 \\
v\vert_{x=0}=t \\
v_{x}\vert_{x=2}=1 \\
v\vert_{t=0}=x+2
\end{cases} 
\end{gather}$$
$$\begin{gather}
v(x,t)=w(x,t)+A(t)x+B(t), \ \text{где } w(0,t)=w_{x}(2,t)=0 \\ 
v_{x}=w_{x}+A(t)\\
v_{t}=w_{t}+A_{t}x+B_{t} \\
v_{xx}=w_{xx}  \\
\begin{cases}
w_{t}+A_{t}x+B_{t}=w_{xx}+3\sin \frac{5\pi x}{4}+1  \\
w(0,t)=0  \\
w_{x}(2,t)=0\\
B(t)=t \\
A(t)=1 \\
w(x,0)+A(0)x+B(0)=x+2 
\end{cases} \Rightarrow \begin{cases}
w_{t}=w_{xx}+3\sin \frac{5\pi x}{4} \\
w(0,t)=0 \\
w_{x}(2,t)=0 \\
w(x,0)+x=x+2
\end{cases}\Rightarrow  \\
\begin{cases}
w_{t}=w_{xx}+3\sin \frac{5\pi x}{4} \\
w(0,t)=0 \\
w_{x}(2,t)=0 \\
w(x,0)=2
\end{cases} 
\end{gather}
$$
$$\begin{gather}
\text{ Вспомогательная задача } \begin{cases}
z_{t}=z_{xx} \\
z\vert_{x=0}=z\vert_{x=2}=0 \\
z\vert_{t=0}=2
\end{cases} \\
z=X(x)T(t) \\
XT'=X''T \\
\frac{T'}{T}=\frac{X''}{X}=-\lambda \\
\begin{cases}
-X''-\lambda X=0 \\
X(0)=X'(2)=0 
\end{cases} \\
X(x)=A\cos \sqrt{ \lambda }x+B\sin \sqrt{ \lambda }x 
\end{gather}$$
$$\begin{gather}
y'(x)=-A\sqrt{ \lambda }\sin \sqrt{ \lambda }x+B\sqrt{ \lambda }\cos \sqrt{ \lambda }x \\
y(0)=0\Rightarrow B=0 \\
y'(2)=0\Rightarrow -A\sqrt{ \lambda }\sin 2\sqrt{ \lambda }=0\Rightarrow  \\
2\sqrt{ \lambda }=\pi k\Rightarrow \lambda_{k}=\left( \frac{\pi k}{2} \right)^2,k\in \mathbb{N} \\
\begin{cases}
\lambda_{n}=\left( \frac{\pi n}{2} \right)^2 \\
X_{n}=\cos\left( \frac{\pi nx}{2} \right)
\end{cases} \\
3\sin\left( \frac{5\pi x}{4} \right)\sim \sum_{n} C_{n}X_{n}  \\
C_{n}=\frac{\int_{0}^23\sin\left( \frac{5\pi x}{4} \right)\cdot \cos\left( \frac{\pi nx}{2} \right)dx}{\int_{0}^2\cos^2\left( \frac{\pi nx}{2} \right)dx} \\
\int_{0}^2\cos^2\left( \frac{\pi nx}{2} \right)dx=\int_{0}^2\cos^2\left( \frac{\pi nx}{2} \right)dx=\int_{0}^2 \frac{\cos(\pi nx)+1}{2}dx= \\
=1+\frac{\sin(2\pi n)}{\pi n}=1 \\
\int_{0}^23\sin\left( \frac{5\pi x}{4} \right)\cdot \cos\left( \frac{\pi nx}{2} \right)dx= \\
=\frac{3}{2}\int_{0}^2\sin\left( \left( \frac{5\pi}{4}+\frac{\pi n}{2} \right)x \right)+\sin\left( \left( \frac{5\pi}{4}-\frac{\pi n}{2} \right)x \right)dx= \\
=-\frac{3}{2}\left( \frac{\cos\left( \left( \frac{5\pi}{4}+\frac{\pi n}{2} \right)\cdot 2 \right)}{\frac{5\pi}{4}+\frac{\pi n}{2}}+ \frac{\cos\left( \left( \frac{5\pi}{4}-\frac{\pi n}{2} \right)\cdot 2 \right)}{\frac{5\pi}{4}-\frac{\pi n}{2}}-\frac{1}{\frac{5\pi}{4}+\frac{\pi n}{2}}-\frac{1}{\frac{5\pi}{4}-\frac{\pi n}{2}}\right) =\\
=\frac{3}{2}\left( -\frac{\cos\left( \frac{5\pi}{2} \right)(-1)^n}{\frac{5\pi}{4}+\frac{\pi n}{2}}- \frac{\cos\left( \frac{5\pi}{2} \right)(-1)^n}{\frac{5\pi}{4}-\frac{\pi n}{2}}+\frac{1}{\frac{5\pi}{4}+\frac{\pi n}{2}}+\frac{1}{\frac{5\pi}{4}-\frac{\pi n}{2}}\right)= \\
=\frac{3}{2}\left(\frac{\frac{5\pi}{2}}{\frac{25\pi^2}{16}-\frac{\pi^2n^2}{4}} \right)=\frac{15\pi}{\frac{25\pi^2}{16}-\frac{\pi^2n^2}{4}} \\
w=\sum _{n=1}^\infty \frac{15\pi}{\frac{25\pi^2}{16}-\frac{\pi^2n^2}{4}}\cdot \cos\left( \frac{\pi nx}{2} \right) 

\end{gather}$$
$$\begin{gather}
v=\sum _{n=1}^\infty \frac{15\pi}{\frac{25\pi^2}{16}-\frac{\pi^2n^2}{4}}\cdot \cos\left( \frac{\pi nx}{2} \right) +x+t \\
u=e^t\left(\sum _{n=1}^\infty \frac{15\pi}{\frac{25\pi^2}{16}-\frac{\pi^2n^2}{4}}\cdot \cos\left( \frac{\pi nx}{2} \right) +x+t\right)
\end{gather}$$



