$$\begin{gather}
x^1\equiv x,\ x^2\equiv y\\
X^1\equiv X,\ X^2\equiv Y\\
(X,Y): \ \begin{cases}
x^1=\frac{1}{2}X^2+\frac{1}{2}\ln Y\\  \\
x^2=\frac{2}{3}X^3-\frac{1}{2}Y
\end{cases}, \ M: \ \begin{pmatrix}
1, & 1
\end{pmatrix},\  \vec{a}: \ \begin{pmatrix}
\frac{3}{2} \\
\frac{3}{2}
\end{pmatrix}
\end{gather}$$

1) $Q^I_{J}=\frac{ \partial x^I }{ \partial X^J }$

$$\begin{gather}
\begin{cases}
\frac{ \partial x^1 }{ \partial X }= X(1,1)=1\\
\frac{ \partial x^1 }{ \partial Y }= \frac{1}{2Y}(1,1)=\frac{1}{2}\\
\frac{ \partial x^2 }{ \partial X }= 2X^2(1,1)=2 \\
\frac{ \partial x^2 }{ \partial X }= -\frac{1}{2}
\end{cases}\Rightarrow Q^I_{J}=\begin{pmatrix}
1 & \frac{1}{2} \\
2 & -\frac{1}{2}
\end{pmatrix} \text{ - матрица перехода}\\
Q=\begin{vmatrix}
1 & \frac{1}{2} \\
2 & -\frac{1}{2}
\end{vmatrix}=-\frac{1}{2}-2\cdot \frac{1}{2}=-\frac{3}{2}\\
P^I_{J}=\frac{ \partial X^I }{ \partial x^J }\\
(P^I_{J})=(Q^I_{J})^{-1}\\
(Q^I_{J})^{-1}=\frac{1}{Q}\begin{pmatrix}
Q_{2}^2 & -Q^1_{2} \\
-Q^2_{1} & Q_{1}^1
\end{pmatrix}=\frac{1}{-\frac{3}{2}}\begin{pmatrix}
-\frac{1}{2} & -\frac{1}{2} \\
-2 & 1
\end{pmatrix}=\frac{2}{3}\begin{pmatrix}
\frac{1}{2} & \frac{1}{2} \\
2 & -1
\end{pmatrix}\\
P^I_{J}=\begin{pmatrix}
\frac{1}{3} & \frac{4}{3} \\
\frac{1}{3} & -\frac{2}{3}
\end{pmatrix} \text{ - обратная матрица перехода}\\
P=\left( \frac{1}{3}\cdot -\frac{2}{3}-\frac{4}{3}\cdot \frac{1}{3} \right)=-\frac{2}{3}=Q^{-1}
\end{gather}$$

2) $\vec{R}_i = Q^j_i \vec{e}_j$

$$\begin{gather}
\vec{R_i} = {Q_i}^1 {\vec{e}}_1 + {Q^2}_i {\vec{e}}_2 
\end{gather}$$

$$\begin{gather}
\begin{cases}
\vec{R_1} = {Q_1}^1 {\vec{e}}_1 + {Q^2}_1 {\vec{e}}_2 = 1 \cdot {\vec{e}}_1 + 2 \cdot {\vec{e}}_2 \\
\vec{R_2} = {Q_2}^1 {\vec{e}}_1 + {Q^2}_2 {\vec{e}}_2 = \frac{1}{2} \cdot {\vec{e}}_1 - \frac{1}{2} \cdot {\vec{e}}_2
\end{cases}
\end{gather}$$

$$\begin{gather}
\vec{R_i} = {Q_i}^1 {\vec{e}}_1 + {Q^2}_i {\vec{e}}_{2} \\
\begin{cases}
\vec{R_{1}} = {Q_{1}}^1 {\vec{e}}_1 + {Q^2}_1 {\vec{e}}_{2} = 1 \cdot {\vec{e}}_1 + 2 \cdot {\vec{e}}_2 \\
\vec{R_{2}} = {Q_2}^1 {\vec{e}}_1 + {Q^2}_2 {\vec{e}}_2 = \frac{1}{2} \cdot {\vec{e}}_1 - \frac{1}{2} \cdot {\vec{e}}_2
\end{cases}
\end{gather}$$

$$\begin{gather}
\vec{R_{i}}=Q_{i}^1{\vec{e}}_{1}+Q^2_{i}{\vec{e}}_{2} \\
\begin{cases}
\vec{R_{1}}=Q_{1}^1{\vec{e}}_{1}+Q^2_{1}{\vec{e}}_{2}= 1\cdot {\vec{e}}_{1}+2\cdot {\vec{e}}_{2} \\
\vec{R_{2}}=Q_{2}^1{\vec{e}}_{1}+Q^2_{2}{\vec{e}}_{2}=\frac{1}{2}\cdot {\vec{e}}_{1}-\frac{1}{2}\cdot {\vec{e}}_{2}
\end{cases}
\end{gather}$$

3) $g_{ij} = \vec{R}_i \cdot \vec{R}_j$

$$\begin{gather}
\begin{cases}
g_{11}=(1\cdot \vec{e}_{1}+2\cdot \vec{e}_{2})(1\cdot \vec{e}_{1}+2\cdot \vec{e}_{2})=1^2+2^2=5\\
g_{12}=(1\cdot \vec{e}_{1}+2\cdot \vec{e}_{2})\left( \frac{1}{2}\vec{e}_{1}-\frac{1}{2}\vec{e}_{2} \right)=\frac{1}{2}-1=-\frac{1}{2}\\
g_{21}=g_{12}=-\frac{1}{2}\\
g_{22}=\left( \frac{1}{2}\vec{e}_{1}-\frac{1}{2}\vec{e}_{2} \right)\left( \frac{1}{2}\vec{e}_{1}-\frac{1}{2}\vec{e}_{2} \right)=\frac{1}{4}+\frac{1}{4}=\frac{1}{2}
\end{cases}\\
g_{IJ}=\begin{pmatrix}
5 & -\frac{1}{2} \\
-\frac{1}{2} & \frac{1}{2}
\end{pmatrix}\\
g=\begin{vmatrix}
5 & -\frac{1}{2} \\
-\frac{1}{2} & \frac{1}{2}
\end{vmatrix}=\frac{5}{2}-\frac{1}{4}=\frac{9}{4}\\
(g^{IJ})=(g_{IJ})^{-1}=\frac{4}{9}\begin{pmatrix}
\frac{1}{2} & \frac{1}{2} \\
\frac{1}{2} & 5
\end{pmatrix}=\begin{pmatrix}
\frac{2}{9} & \frac{2}{9} \\
\frac{2}{9} & \frac{20}{9}
\end{pmatrix}\\
q^{IJ}=g^{IJ}\\
q=\frac{16}{81}\cdot \left( \frac{5}{2}-\frac{1}{4} \right)=\frac{16}{81}\cdot \frac{9}{4}=\frac{4}{9}\\
qg=1
\end{gather}$$

4) $\overrightarrow{R^i}=g^{ij}\overrightarrow{R_{j}}$

$$\begin{gather}
\overrightarrow{R^i}=g^{i1}\overrightarrow{R_{1}}+g^{i 2}\overrightarrow{R_{2}} \\
\begin{cases}
\overrightarrow{R^1}=g^{11}\overrightarrow{R_{1}}+g^{12}\overrightarrow{R_{2}}=\frac{2}{9}(1\cdot \vec{e}_{1}+2\cdot \vec{e}_{2})+\frac{2}{9}\left( \frac{1}{2}\vec{e}_{1}-\frac{1}{2}\vec{e}_{2} \right)=\frac{1}{3}\vec{e}_{1}+\frac{1}{3}\vec{e}_{2} \\
\overrightarrow{R^2}=g^{21}\overrightarrow{R_{1}}+g^{22}\overrightarrow{R_{2}}=\frac{2}{9}\left( \vec{e}_{1}+2\vec{e}_{2} \right)+\frac{20}{9}\left( \frac{1}{2}\vec{e}_{1}-\frac{1}{2}\vec{e}_{2}\right)=\frac{4}{3}\vec{e}_{1} -\frac{2}{3}\vec{e}_{2}
\end{cases}
\end{gather}$$

5) $\vec{a}=a^I\vec{e}_{I}=b^I\vec{R}_{I}=b_{I}\vec{R}^I$

$$\begin{gather}
b^I=P^I_{J}a^J=P^I_{1}a^1+P^I_{2}a^2 \\
\begin{cases}
b^1= \frac{1}{3}\cdot \frac{3}{2}+\frac{1}{3}\cdot \frac{3}{2} =1\\
b^2=\frac{4}{3}\cdot \frac{3}{2}-\frac{2}{3}\cdot \frac{3}{2}=1 
\end{cases}\\
b_{I}=Q_{I}^Ja_{J}=Q^J_{I}\delta_{JK}a^K=Q_{I}^1\cdot a^1+Q_{I}^2\cdot a^2 \\
\begin{cases}
b_{1}=1\cdot \frac{3}{2}+2\cdot \frac{3}{2}=\frac{9}{2} \\
b_{2} =\frac{1}{2}\cdot \frac{3}{2}-\frac{1}{2}\cdot \frac{3}{2}=0
\end{cases}
\end{gather}$$

Проверка:
$$\begin{gather}
\overrightarrow{R^I}\cdot \overrightarrow{R_{J}}=\delta^I_{J} \\
\begin{cases}
\overrightarrow{R^1}\cdot \overrightarrow{R_{1}}=\begin{pmatrix}
\frac{1}{3} & \frac{1}{3}
\end{pmatrix}\circ\begin{pmatrix}
1 \\
2 
\end{pmatrix}=\frac{1}{3}+\frac{2}{3}=1=\delta_{1}^1 \\
\overrightarrow{R^1}\cdot \overrightarrow{R_{2}}=\begin{pmatrix}
\frac{1}{3} & \frac{1}{3} 
\end{pmatrix} \circ\begin{pmatrix}
\frac{1}{2} \\
-\frac{1}{2}
\end{pmatrix}=0=\delta^1_{2} \\
\overrightarrow{R^2}\cdot \overrightarrow{R_{1}}=\begin{pmatrix}
\frac{4}{3} & -\frac{2}{3}
\end{pmatrix}\circ\begin{pmatrix}
1 \\
2
\end{pmatrix}=\frac{4}{3}-\frac{4}{3}=0=\delta^2_{1} \\
\overrightarrow{R^2}\cdot \overrightarrow{R_{2}}=\begin{pmatrix}
\frac{4}{3} & -\frac{2}{3}
\end{pmatrix}\circ\begin{pmatrix}
\frac{1}{2} \\
-\frac{1}{2}
\end{pmatrix}=\frac{2}{3}+\frac{1}{3}=1=\delta^2_{2}
\end{cases} 
\end{gather}$$
	
$$\begin{gather}

g_{IJ}=Q_{I}^KQ_{J}^L\delta_{KL}=Q_{I}^1\cdot Q_{J}^1+Q_{I}^2\cdot Q_{J}^2 \\
\begin{cases}
g_{11}=1\cdot 1+2\cdot 2=5 \\
g_{12}=1\cdot \frac{1}{2}+2\cdot -\frac{1}{2}=-\frac{1}{2}  \\
g_{21}=g_{21} \\
g_{22}=\frac{1}{2}\cdot \frac{1}{2}+ -\frac{1}{2}\cdot -\frac{1}{2}=\frac{1}{2}
\end{cases} \\
g^{IJ}=P^I_{K}P^J_{L}\delta^{KL}=P^I_{1}\cdot P^J_{1}+P^I_{2}\cdot P^J_{2} \\
\begin{cases}
g^{11}=\frac{1}{3}\cdot \frac{1}{3}+\frac{1}{3}\cdot \frac{1}{3}=\frac{2}{9} \\
g^{12}=\frac{1}{3}\cdot \frac{4}{3}+\frac{1}{3}\cdot -\frac{2}{3}=\frac{2}{9} \\
g^{21}=g^{12} \\
g^{22}=\frac{4}{3}\cdot \frac{4}{3}+ -\frac{2}{3}\cdot -\frac{2}{3}=\frac{20}{9}
\end{cases} \\
g^{IJ}=\overrightarrow{R^I}\cdot \overrightarrow{R^J} \\
\begin{cases}
g^{11}=\begin{pmatrix}
\frac{1}{3} & \frac{1}{3}
\end{pmatrix}\circ \begin{pmatrix}
\frac{1}{3} \\
\frac{1}{3}
\end{pmatrix}=\frac{2}{9} \\
g^{12}=\begin{pmatrix}
\frac{1}{3} & \frac{1}{3}
\end{pmatrix}\circ\begin{pmatrix}
\frac{4}{3} \\
-\frac{2}{3}
\end{pmatrix}=\frac{2}{9} \\
g^{21}=g^{12} \\
g^{22}=\begin{pmatrix}
\frac{4}{3} & -\frac{2}{3}
\end{pmatrix}\circ \begin{pmatrix}
\frac{4}{3} \\
-\frac{2}{3}
\end{pmatrix}=\frac{20}{9}
\end{cases}
\end{gather}$$

$$\begin{gather}
\vec{R}_{J}=g_{IJ}\vec{R}^I =g_{1J}\vec{R}^1+g_{2J}\vec{R}^2\\
\begin{cases}
\vec{R}_{1}=5\cdot\left( \frac{1}{3}\vec{e}_{1}+ \frac{1}{3}\vec{e}_{2}\right)+ -\frac{1}{2}\cdot \left( \frac{4}{3}\vec{e}_{1} -\frac{2}{3}\vec{e}_{2}\right)=\left( \frac{5}{3}-\frac{2}{3} \right)\vec{e}_{1}+\left( \frac{5}{3}+\frac{1}{3} \right)\vec{e}_{2}=\vec{e}_{1}+2\vec{e}_{2} \\
\vec{R}_{2}=-\frac{1}{2}\cdot \left( \frac{1}{3}\vec{e}_{1}+\frac{1}{3}\vec{e}_{2} \right)+\frac{1}{2}\cdot \left( \frac{4}{3}\vec{e}_{1}-\frac{2}{3}\vec{e}_{2} \right)=\left( -\frac{1}{6}+\frac{2}{3} \right)\vec{e}_{1}+\left( -\frac{1}{6}-\frac{1}{3} \right)\vec{e}_{2}=\frac{1}{2}\vec{e}_{1}-\frac{1}{2}\vec{e}_{2}
\end{cases} \\
b_{I}=g_{IJ}b^J=g_{I1}b^1+g_{I 2}b^2 \\
\begin{cases}
b_{1}=5 -\frac{1}{2}=\frac{9}{2} \\
b_{2} =-\frac{1}{2}+\frac{1}{2}=0
\end{cases} \\
b^I=g^{IJ}b_{J}=g^{I1}b_{1}+g^{I 2}b_{2} \\
\begin{cases}
b^1=\frac{2}{9}\cdot \frac{9}{2}+0=1 \\
b^2=\frac{2}{9}\cdot \frac{9}{2}=1
\end{cases} \\
b_I=\vec{a}\cdot \vec{R}_{I} \\
b^I=\vec{a}\cdot \vec{R}^I\\
\begin{cases}
b_1=\begin{pmatrix}
1 & 2
\end{pmatrix}\circ\begin{pmatrix}
\frac{3}{2} \\
\frac{3}{2}
\end{pmatrix}=\frac{9}{2} \\
b_2=\begin{pmatrix}
\frac{1}{2} & -\frac{1}{2}
\end{pmatrix}\circ\begin{pmatrix}
\frac{3}{2} \\
\frac{3}{2}
\end{pmatrix}=0 \\
b^{1}=\begin{pmatrix}
\frac{1}{3} & \frac{1}{3}
\end{pmatrix}\circ \begin{pmatrix}
\frac{3}{2} \\
\frac{3}{2}
\end{pmatrix}=1 \\
b^{2}=\begin{pmatrix}
\frac{4}{3} & -\frac{2}{3}
\end{pmatrix}\circ\begin{pmatrix}
\frac{3}{2} \\
\frac{3}{2}
\end{pmatrix}=1
\end{cases}
\end{gather}$$









