#### Задание 1
Дано:
$$\begin{gather}
f(t)= \frac{\operatorname{ ch } (\alpha t)-\cos(\beta t)}{t}
\end{gather}$$
Найти:
$$F(p)\;(f(t)\doteqdot F(p)),\int _{0}^t \frac{\operatorname{ ch } (\alpha \tau)-\cos(\beta \tau)}{\tau}d\tau$$
Решение:
$$\begin{gather}
\frac{q(t)}{t}\doteqdot \int _{p}^{+\infty }Q(w)dw \\
q(t)=\operatorname{ ch } (\alpha t)-\cos(\beta t)\doteqdot \frac{p}{p^2-\alpha^2}-\frac{p}{p^2+\beta^2}=Q(p) \\
\int _{p}^{+\infty}\left( \frac{w}{w^2-\alpha^2}-\frac{w}{w^2+\beta^2} \right)dw= \left. \frac{1}{2}(\ln(w^2-\alpha^2)-\ln(w^2+\beta^2)) \right\rvert_{p}^{+\infty}= \\
\int \frac{w}{w^2+C}dw=\frac{1}{2}\int \frac{d(w^2+C)}{w^2+C}=\frac{1}{2}\ln(w^2+C)+C_{2} \\
=\frac{1}{2}\left. \ln\left( \frac{w^2-\alpha^2}{w^2+\beta^2} \right) \right\rvert _{p}^{+\infty}=\frac{1}{2}\left( 0-\ln\left( \frac{p^2-\alpha^2}{p^2+\beta^2} \right) \right) \\
f(t)=\frac{q(t)}{t}\doteqdot F(p)=-\frac{1}{2}\ln\left( \frac{p^2-\alpha^2}{p^2+\beta^2} \right) \\
\int _{0}^t f(\tau)d\tau\doteqdot \frac{F(p)}{p}
\end{gather}$$
#### Задание 2
Решение:
$$\begin{gather}
\frac{p}{(p-1)(p^2+1)}\doteqdot  \\
\frac{p}{(p-1)(p^2+1)}=\frac{A}{p-1}+\frac{Bp+C}{p^2+1}=\frac{A(p^2+1)+(Bp+C)(p-1)}{(p-1)(p^2+1)}=\frac{1}{2}\left( \frac{1}{p-1}+\frac{-p}{p^2+1} +\frac{1}{p^2+1}\right) \\
1=2A \Rightarrow A=\frac{1}{2}\\
i+0=(Bi+C)(i-1)=-B-C+i(C-B)\Rightarrow \begin{cases}
B+C=0 \\
C-B=1
\end{cases}\Rightarrow C=\frac{1}{2},B=-\frac{1}{2} \\
e^{\alpha t}f(t)\doteqdot F(p-\alpha) \\
\frac{1}{2}\left( \frac{1}{p-1}-\frac{p}{p^2+1} +\frac{1}{p^2+1}\right)\doteqdot \frac{1}{2}(e^t -\cos t+\sin t) \\
\frac{p}{(p-1)(p^2+1)}=\frac{1}{p-1}\cdot \frac{p}{p^2+1}\doteqdot \int _{0}^{t} e^{t-\tau}\cos(\tau)d\tau = e^t\int _{0}^t\cos(x)d(-e^{-x})= \\
=e^t\left(-\left. e^{-x}\cos x \right\rvert _{0}^t- \int _{0}^t-e^{-x}\cdot -\sin xdx \right)=-\cos t+e^t-e^t\int _{0}^t \sin xd(-e^{-x})= \\
=-\cos t+e^t-e^t\left( \left. -e^{-x}\sin x \right\rvert _{0}^t-\int _{0}^t -e^{-x}\cos xdx \right)=-\cos t+e^t+\sin t-e^t\int _{0}^t \cos xe^{-x}dx \\
A=e^t\int _{0}^t \cos xe^{-x}dx \Rightarrow \\
A=-\cos t+e^t+\sin t-A\Rightarrow  \\
A=\frac{1}{2}(-\cos t+e^t+\sin t)
\end{gather}$$
$$\begin{gather}
F(p)=\frac{p}{(p-1)(p^2+1)}, F(p)\doteqdot f(t)=\frac{1}{2}(e^t-\cos t+\sin t) \\
F_{1}(p)=\frac{F(p)}{p}\doteqdot \int _{0}^t f(\tau)d\tau=\frac{1}{2}((e^t-1)+(-\sin t)+(1-\cos t))=\frac{1}{2}(e^t-\cos t-\sin t)=f_{1}(t) \\
\frac{F_{1}(p)}{p}\doteqdot \int _{0}^t f_{1}(\tau)d\tau=\frac{1}{2}(e^t-1-\sin t+\cos t-1)=\frac{1}{2}(e^t+\cos t-\sin t-2)
\end{gather}$$
#### Задание 3
Дано:
$$\begin{gather}
\begin{cases}
x''+y'=0 \\
y''+x'=1-2\sin t \\
x(0)=1 \\
y(0)=1 \\
x'(0)=1 \\
y'(0)=1
\end{cases}
\end{gather}$$
Решение:
$$\begin{gather}
\begin{vmatrix}
x(t)\doteqdot X(p) \\
x'(t)\doteqdot pX(p)-X(0)=pX(p)-1 \\
x''(t)\doteqdot p^2X(p)-px(0)-x'(0)=p^2X(p)-p-1 \\
y(t)\doteqdot Y(p) \\
y'(t)\doteqdot pY(p)-y(0)=pY(p)-1 \\
y''(t)\doteqdot p^2Y(p)-py(0)-y'(0)=p^2Y(p)-p-1  \\
0\doteqdot 0\\
1-2\sin t\doteqdot \frac{1}{p}-2 \frac{1}{p^2+1}
\end{vmatrix} \\
\begin{cases}
p^2X-p-1+pY-1=0 \\
p^2Y-p-1+pX-1=\frac{1}{p}-2 \frac{1}{p^2+1}
\end{cases} 
\end{gather}$$
$$\begin{gather}
\begin{cases}
p^2X+pY=p+2 \\
pX+p^2Y=p+2+\frac{1}{p}-\frac{2}{p^2+1}
\end{cases} \\
\begin{cases}
pX=\frac{1}{p}(-pY+p+2) \\
(-1+p^2)Y+1+\frac{2}{p}=p+2+\frac{1}{p}-\frac{2}{p^2+1} 
\end{cases}  \\
Y=\frac{1}{p^2-1}\left( p+1-\frac{1}{p}-\frac{2}{p^2+1} \right) \\
Y=\frac{1}{p-1}-\frac{p^2+2p+1}{p(p^2-1)(p^2+1)} \\
Y=\frac{1}{p-1}-\frac{p+1}{p(p-1)(p^2+1)} \\
Y=\frac{p^3+p-p-1}{p(p-1)(p^2+1)}=\frac{p^2+p+1}{p(p^2+1)}=\frac{1}{p}+\frac{1}{p^2+1} \\
X=\frac{1}{p^2}\left( -1-\frac{p}{p^2+1}+p+2 \right)=\frac{1}{p^2}\left( -\frac{p}{p^2+1}+p+1 \right)= 
\end{gather}$$
$$\begin{gather}
=\frac{1}{p^2} \frac{p^3+p^2+1}{p^2+1}=\frac{p}{p^2+1}+\frac{1}{p^2} \\
\begin{cases}
X=\frac{p}{p^2+1}+\frac{1}{p^2} \\
Y=\frac{1}{p}+\frac{1}{p^2+1}
\end{cases}\Rightarrow \begin{cases}
x=\cos t+t \\
y=1+\sin t
\end{cases}
\end{gather}$$

#### Задание 4
Дано:
$$\begin{gather}
\Gamma(n)=\int _{0}^\infty x^{n-1}e^{-x}dx \\
B(a,b)=\int _{0}^1 x^{a-1}(1-x)^{b-1}dx=\frac{\Gamma(a)\Gamma(b)}{\Gamma(a+b)}
\end{gather}$$
Решение:
$$\begin{gather}
\int _{0}^1 \frac{x^{\frac{11}{3}}}{\sqrt[3]{ 1-x^2  }}dx=\begin{vmatrix}
x=\sin\varphi  \\
dx=\cos\varphi d\varphi 
\end{vmatrix}=\int _{0}^{\frac{\pi}{2}}\sin ^{\frac{11}{3}}\varphi \cos ^{\frac{1}{3}}\varphi d\varphi =\frac{1}{2}2\int _{0}^{\frac{\pi}{2}} \sin ^{2b-1}\varphi \cos ^{2a-1}\varphi d\varphi =\frac{1}{2}B\left( \frac{7}{3},\frac{2}{3} \right) \\
2a-1=\frac{11}{3}\Rightarrow a=\frac{1}{2} \frac{14}{3}=\frac{7}{3} \\
2b-1=\frac{1}{3}\Rightarrow b=\frac{2}{3}\\
0.403067
\end{gather}$$
#### Задание 5
Дано:
$$\begin{gather}
F(p)=\frac{p^2+1}{(p^2-1)^2}
\end{gather}$$
Найти:
$$\begin{gather}

\end{gather}$$
Решение:
$$\begin{gather}

\end{gather}$$
#### Задание 6
Дано:
$$\begin{gather}
f(t) = \begin{cases}\dfrac{h}{\tau}t,& t\in \left[ 0,\tau\right] \\ -\dfrac{h}{\tau}\left( t-2\tau\right), & t \in \left(\tau,2\tau\right]\end{cases}, T=2\tau
\end{gather}$$
Решение:
$$\begin{gather}
F(p)=\frac{F_{0}(p)}{1-e^{-Tp}}=\frac{h}{\tau p^2} (1-e^{-\tau p}) \\
F_{0}(p)=\frac{h}{\tau p^2} (1-e^{-\tau p})^2 \\
\int _{0}^\tau  \frac{h}{\tau}t e^{-pt}dt+\int _{\tau}^{2\tau} -\frac{h}{\tau}(t-2\tau)e^{-pt}dt=\frac{h}{\tau p^2} (1-e^{-\tau p})^2
\end{gather}$$
#### Задание 7
Дано:
$$\begin{gather}
x''-x'-6x={e}^{-t}, \ x\left( 0 \right)=0, \ {x}'\left( 0 \right)=-1
\end{gather}$$
Решение:
$$\begin{gather}
x(t)\doteqdot X(p) \\
x'(t)\doteqdot pX(p)-x(0)=pX \\
x''\doteqdot p^2X(p)-px(0)-x'(0)=p^2X+1 \\
e^{-t}\doteqdot \frac{1}{p+1} \\
p^2X+1-pX-6X=\frac{1}{p+1} \\
X=-\frac{1}{p^2-p-6} \frac{p}{p+1}=-\frac{p}{(p+1)(p+2)(p-3)} \\
-p=A(p+2)(p-3)+B(p+1)(p-3)+C(p+1)(p+2) \\
1=-4A\Rightarrow A=-\frac{1}{4} \\
2=5B\Rightarrow B=\frac{2}{5} \\
-3=20C\Rightarrow C=-\frac{3}{20} \\
X=\frac{A}{p+1}+\frac{B}{p+2}+\frac{C}{p-3} \\
x=Ae^-t+Be^{-2t}+Ce^{3t}
\end{gather}$$

#### Задание 8
Дано:
$$\begin{gather}
y'' + y = \frac{1}{\cos \left( t \right) + 2},y(0)=0, y'(0)=0
\end{gather}$$
Решение:
$$\begin{gather}
y\doteqdot Y \\
y''\doteqdot p^2Y \\
\frac{1}{\cos t+2}
\end{gather}$$












