$$\begin{gather}
w= \operatorname{ th } z \\
z_{0}=\ln(4) - \frac{i\pi}{3} \\

\end{gather}$$
Изи

$$\begin{gather}
\sum_{i=1}^{\infty} \frac{(z-2+i)^n}{(3i)^n(n+1)\ln(n+1)} \\
x=z+2-i \\
\sum_{i=1}^{\infty} (-i)^n\frac{x^n}{3^n(n+1)\ln(n+1)} \\
y=-\frac{x}{3} \\
\sum_{i=1}^{\infty} i^n \frac{y^n}{(n+1)\ln(n+1)}=i\sum_{i=0}^{\infty}(-1)^{n} \frac{y^{2n+1}}{(2n+2)\ln(2n+2)}+\sum_{i=1}^{\infty} (-1)^n \frac{y^{2n}}{(2n+1)\ln(2n+1)} \\
i \frac{y}{2\cdot \ln 2}-\frac{y^2}{3\cdot \ln 3}-i \frac{y^{3}}{4\cdot  \ln 4}+\frac{y^4}{5\cdot \ln 5}+\ldots=i\left( \frac{y}{2\cdot \ln 2}-\frac{y^3}{4\cdot \ln 4}+\ldots \right)+\left( -\frac{y^2}{3\cdot \ln 3}+\frac{y^4}{5\cdot \ln 5} \right) \\
\int _{0}^\infty (-i)^n \frac{y^n}{(n+1)\ln(n+1)}dy=(-i)^n  \\

\end{gather}$$
$$\begin{gather}
\frac{y^{n}}{(n+1)\ln(n+1)}\to 0 \\
\lvert y \rvert <1 \\
 
\end{gather}$$
